src/parser/desugar.fs
@@ -1,21 +1,23 @@
 (*
-   Copyright 2008-2014 Nikhil Swamy and Microsoft Research
+  Copyright 2008-2014 Nikhil Swamy and Microsoft Research
 
-   Licensed under the Apache License, Version 2.0 (the "License");
-   you may not use this file except in compliance with the License.
-   You may obtain a copy of the License at
+  Licensed under the Apache License, Version 2.0 (the "License");
+  you may not use this file except in compliance with the License.
+  You may obtain a copy of the License at
 
-       http://www.apache.org/licenses/LICENSE-2.0
+  http://www.apache.org/licenses/LICENSE-2.0
 
-   Unless required by applicable law or agreed to in writing, software
-   distributed under the License is distributed on an "AS IS" BASIS,
-   WITHOUT WARRANTIES OR CONDITIONS OF ANY KIND, either express or implied.
-   See the License for the specific language governing permissions and
-   limitations under the License.
+  Unless required by applicable law or agreed to in writing, software
+  distributed under the License is distributed on an "AS IS" BASIS,
+  WITHOUT WARRANTIES OR CONDITIONS OF ANY KIND, either express or implied.
+  See the License for the specific language governing permissions and
+  limitations under the License.
 *)
 #light "off"
 module Microsoft.FStar.Parser.Desugar
+
 open Microsoft.FStar
+open Microsoft.FStar.Parser
 open Microsoft.FStar.Range
 open Microsoft.FStar.Parser.AST
 open Microsoft.FStar.Parser.DesugarEnv
@@ -40,7 +42,7 @@ let mk_app e args =
       | Inr e' -> 
         ewithpos (Exp_app(e, e')) (Range.union_ranges e.p e'.p))
     e args 
-     
+    
 let mk_tapp t args =
   List.fold_left
     (fun t -> function
@@ -50,54 +52,55 @@ let mk_tapp t args =
         Typ_meta (Meta_pos(Typ_dep(t, e), Range.union_ranges (tpos t) e.p)))
     t args 
 
-let op_as_vlid (env:env) arity r s = 
+let op_as_vlid (env:env) arity r s =
   let r l = Some <| set_lid_range l r in
-    match s, env.phase with 
-      | "=", _ ->    r Const.op_Eq
-      | ":=", _ ->   r Const.op_ColonEq
-      | "<", _ ->    r Const.op_LT
-      | "<=", _ ->   r Const.op_LTE
-      | ">", _ ->    r Const.op_GT
-      | ">=", _ ->   r Const.op_GTE
-      | "&&", _ ->   r Const.op_And
-      | "||", _ ->   r Const.op_Or
-      | "*", Expr -> r Const.op_Multiply
-      | "*", _ ->    r Const.mul_lid
-      | "+", Expr -> r Const.op_Addition
-      | "+", _ ->    r Const.add_lid
-      | "-", Expr when (arity=1) -> r Const.op_Minus
-      | "-", _ when (arity=1) -> r Const.minus_lid
-      | "-", Expr -> r Const.op_Subtraction
-      | "-", _ ->    r Const.sub_lid
-      | "/", Expr -> r Const.op_Division
-      | "/", _ ->    r Const.div_lid
-      | "%", Expr -> r Const.op_Modulus
-      | "%", _ ->    r Const.modulo_lid
-      | "!", _ ->    r Const.read_lid
-      | "@", _ ->    r Const.list_append_lid
-      | "^", _ ->    r Const.string_concat_lid
-      | "|>", _ ->   r Const.pipe_right_lid
-      | "<|", _ ->   r Const.pipe_left_lid
-      | _ -> None
+  match s, env.phase with
+    | "=", _ ->    r Const.op_Eq
+    | ":=", _ ->   r Const.op_ColonEq
+    | "<", _ ->    r Const.op_LT
+    | "<=", _ ->   r Const.op_LTE
+    | ">", _ ->    r Const.op_GT
+    | ">=", _ ->   r Const.op_GTE
+    | "&&", _ ->   r Const.op_And
+    | "||", _ ->   r Const.op_Or
+    | "*", Expr -> r Const.op_Multiply
+    | "*", _ ->    r Const.mul_lid
+    | "+", Expr -> r Const.op_Addition
+    | "+", _ ->    r Const.add_lid
+    | "-", Expr when (arity=1) -> r Const.op_Minus
+    | "-", _ when (arity=1) -> r Const.minus_lid
+    | "-", Expr -> r Const.op_Subtraction
+    | "-", _ ->    r Const.sub_lid
+    | "/", Expr -> r Const.op_Division
+    | "/", _ ->    r Const.div_lid
+    | "%", Expr -> r Const.op_Modulus
+    | "%", _ ->    r Const.modulo_lid
+    | "!", _ ->    r Const.read_lid
+    | "@", _ ->    r Const.list_append_lid
+    | "^", _ ->    r Const.string_concat_lid
+    | "|>", _ ->   r Const.pipe_right_lid
+    | "<|", _ ->   r Const.pipe_left_lid
+    | "<>", _ ->   r Const.op_notEq
+    | _ -> None
 
-let op_as_tylid r s = 
+let op_as_tylid r s =
   let r l = Some <| set_lid_range l r in
-    match s with 
-      | "=" ->    r Const.eq2_lid
-      | "<>" ->   r Const.neq2_lid
-      | "<" ->    r Const.lt_lid
-      | "<=" ->   r Const.lte_lid
-      | ">" ->    r Const.gt_lid
-      | ">=" ->   r Const.gte_lid
-      | "/\\" ->  r Const.and_lid
-      | "\\/" ->  r Const.or_lid
-      | "==>" ->  r Const.implies_lid
-      | "<==>" -> r Const.iff_lid 
-      | _ -> None
+  match s with
+    | "=" ->    r Const.eq2_lid
+    | "<>" ->   r Const.neq2_lid
+    | "<" ->    r Const.lt_lid
+    | "<=" ->   r Const.lte_lid
+    | ">" ->    r Const.gt_lid
+    | ">=" ->   r Const.gte_lid
+    | "/\\" ->  r Const.and_lid
+    | "\\/" ->  r Const.or_lid
+    | "==>" ->  r Const.implies_lid
+    | "<==>" -> r Const.iff_lid
+    | _ -> None
 
-let rec is_type env (t:term) = 
+let rec is_type env (t:term) =
   if t.level = Type then true
-  else match t.term with 
+  else match t.term with
     | Wild -> true
     | Op("*", hd::_)                    (* tuple constructor *)
     | Op("=", hd::_) -> is_type env hd  (* equality predicate *)
@@ -105,213 +108,229 @@ let rec is_type env (t:term) =
     | Op("<=", _)
     | Op(">", _)
     | Op(">=", _) -> env.phase = Formula
-    | Op(s, _) -> (match op_as_tylid t.range s with None -> false | _ -> true)
+    | Op(s, _) -> (match op_as_tylid t.range s with
+        | None -> false
+        | _ -> true)
     | QForall _
     | QExists _
     | Sum _
     | Refine _
     | Tvar _ -> true
     | Var l
-    | Name l 
+    | Name l
     | Construct(l, _) -> is_type_lid env l
     | Abs(_, t)
-    | App(t, _) 
-    | Paren t 
-    | Ascribed(t, _) 
+    | App(t, _)
+    | Paren t
+    | Ascribed(t, _)
     | Product(_, t)  -> is_type env t
     | _ -> false
 
-let rec is_kind (t:term) : bool = 
-  if t.level = Kind 
+let rec is_kind (t:term) : bool =
+  if t.level = Kind
   then true
-  else match t.term with 
+  else match t.term with
     | Name {str="P"}
     | Name {str="S"}
-    | Name {str="E"} -> true
+    | Name ({str="E"}) -> true
     | Product(_, t) -> is_kind t
-    | Paren t -> is_kind t 
+    | Paren t -> is_kind t
     | _ -> false
 
-let rec is_type_binder env b = 
+let rec is_type_binder env b =
   if b.level = Formula
-  then match b.binder with 
-    | Variable _ 
+  then match b.binder with
+    | Variable _
     | Annotated _ -> false
     | TAnnotated _
     | TVariable _ -> true
     | NoName t -> is_kind  t
-  else match b.binder with 
+  else match b.binder with
     | Variable _ -> raise (Error("Unexpected binder without annotation", b.range))
-    | TVariable _ -> false 
-    | TAnnotated _ -> true 
-    | Annotated (_, t) 
+    | TVariable _ -> false
+    | TAnnotated _ -> true
+    | Annotated (_, t)
     | NoName t -> is_kind t
 
-let sort_ftv ftv = 
+let sort_ftv ftv =
   Util.sort_with (fun x y -> String.compare x.idText y.idText) <|
       Util.remove_dups (fun x y -> x.idText = y.idText) ftv
 
 let rec free_type_vars_b env binder = match binder.binder with
   | Variable x -> env, []
-  | TVariable x -> 
-    let env, _ = push_local_tbinding env x in 
+  | TVariable x ->
+    let env, _ = push_local_tbinding env x in
     (env, [x])
-  | Annotated(id, term) -> 
+  | Annotated(id, term) ->
     (env, free_type_vars env term)
-  | TAnnotated(id, term) -> 
+  | TAnnotated(id, term) ->
     let env, _ = push_local_tbinding env id in
     (env, [])
-  | NoName t -> 
+  | NoName t ->
     (env, free_type_vars env t)
-and free_type_vars env t = match t.term with 
-  | Tvar a -> 
-    (match DesugarEnv.try_lookup_typ_var env a with 
+and free_type_vars env t = match t.term with
+  | Tvar a ->
+    (match DesugarEnv.try_lookup_typ_var env a with
       | None -> [a]
       | _ -> [])
 
-  | Wild      
-  | Const _ 
+  | Wild
+  | Const _
   | Var  _
   | Name _  -> []
 
   | Paren t
   | Ascribed(t, _) -> free_type_vars env t
 
-  | Construct(_, ts) 
+  | Construct(_, ts)
   | Op(_, ts) -> List.collect (free_type_vars env) ts
 
   | App(t1,t2) -> free_type_vars env t1@free_type_vars env t2
 
-  | Refine (b, t) -> 
-    let env, f = free_type_vars_b env b in 
+  | Refine (b, t) ->
+    let env, f = free_type_vars_b env b in
     f@free_type_vars env t
       
-  | Product(binders, body)  
+  | Product(binders, body)
   | Sum(binders, body) ->
-    let env, free = List.fold_left (fun (env, free) binder -> 
-      let env, f = free_type_vars_b env binder in 
-      env, f@free) (env, []) binders in 
+    let env, free = List.fold_left (fun (env, free) binder ->
+      let env, f = free_type_vars_b env binder in
+      env, f@free) (env, []) binders in
     free@free_type_vars env body
 
   | Abs _  (* not closing implicitly over free vars in type-level functions *)
-  | If _ 
+  | If _
   | QForall _
   | QExists _ -> [] (* not closing implicitly over free vars in formulas *)
   | Let _
   | Affine _
   | Project  _
-  | Record _  
+  | Record _
   | Match _
-  | Seq _ -> error "Unexpected type in free_type_vars computation" t t.range 
+  | TryWith _
+  | Seq _ -> error "Unexpected type in free_type_vars computation" t t.range
     
-let close env t = 
+let close env t =
   let ftv = sort_ftv <| free_type_vars env t in
-  if List.length ftv = 0 
+  if List.length ftv = 0
   then t
-  else let binders = ftv |> List.map (fun x -> mk_binder (TAnnotated(x, kind_star x.idRange)) x.idRange Type) in 
-       let result = mk_term (Product(binders, t)) t.range t.level in 
-    (* let _ = pr "Implicitly closed type at %s to %s\n" (Range.string_of_range result.range) (term_to_string result) in *)
+  else let binders = ftv |> List.map (fun x -> mk_binder (TAnnotated(x, kind_star x.idRange)) x.idRange Type) in
+       let result = mk_term (Product(binders, t)) t.range t.level in
+       (* let _ = pr "Implicitly closed type at %s to %s\n" (Range.string_of_range result.range) (term_to_string result) in *)
        result
-  
+         
 let rec is_app_pattern p = match p.pattern with
   | PatAscribed(p,_) -> is_app_pattern p
   | PatApp({pattern=PatVar id}, _) -> true
   | _ -> false
 
 let rec destruct_app_pattern p = match p.pattern with
-  | PatAscribed(p,t) -> 
-    let (name, args, _) = destruct_app_pattern p in 
+  | PatAscribed(p,t) ->
+    let (name, args, _) = destruct_app_pattern p in
     (name, args, Some t)
-  | PatApp({pattern=PatVar id}, args) -> 
+  | PatApp({pattern=PatVar id}, args) ->
     (id, args, None)
-  | _ -> 
+  | _ ->
     failwith "Not an app pattern"
 
-let rec desugar_data_pat env (p:pattern) : (env * either<(btvdef*kind), (bvvdef*typ)> * Syntax.pat) = 
+let rec desugar_data_pat env (p:pattern) : (env * either<(btvdef*kind), (bvvdef*typ)> * Syntax.pat) =
   match p.pattern with
-    | PatOr (p::ps) -> 
-      let env0 = env in 
+    | PatOr (p::ps) ->
+      let env0 = env in
       let q = p in
-      let env, var, p = desugar_data_pat env p in 
-      let ps = List.map (fun p -> 
-        let _, _, p = desugar_data_pat env0 p in 
+      let env, var, p = desugar_data_pat env p in
+      let ps = List.map (fun p ->
+        let _, _, p = desugar_data_pat env0 p in
         p) ps in
-      let pat = Pat_disj (p::ps) in 
+      let pat = Pat_disj (p::ps) in
       ignore (check_pat_vars q.range pat);
       env, var, pat
 
     | PatAscribed(p, t) ->
-      let (env, binder, p) = desugar_data_pat env p in 
-      let binder = match binder with 
+      let (env, binder, p) = desugar_data_pat env p in
+      let binder = match binder with
         | Inl (x, _) -> Inl(x, desugar_kind env t)
         | Inr (x, _) -> Inr(x, desugar_typ env t) in
       (env, binder, p)
 
     | PatTvar a ->
-      if a.idText = "'_"  
+      if a.idText = "'_"
       then (env, Inl(new_bvd (Some p.range), Kind_unknown), Pat_twild)
       else let env, abvd = push_local_tbinding env a in
            (env, Inl(abvd, Kind_unknown), Pat_tvar abvd)
 
-    | PatWild -> 
+    | PatWild ->
       let x = new_bvd (Some p.range) in
       (env, Inr(x, Typ_unknown), Pat_wild)
         
-    | PatConst c -> 
+    | PatConst c ->
       let x = new_bvd (Some p.range) in
       (env, Inr(x, Typ_unknown), Pat_constant c)
 
-    | PatVar x -> 
-      let env, xbvd = push_local_vbinding env x in 
+    | PatVar x ->
+      let env, xbvd = push_local_vbinding env x in
       (env, Inr(xbvd, Typ_unknown), Pat_var xbvd)
 
-    | PatName l -> 
+    | PatName l ->
       let _ = fail_or (try_lookup_datacon env) l in
       let x = new_bvd (Some p.range) in
       (env, Inr(x, Typ_unknown), Pat_cons(l, []))
 
     | PatApp({pattern=PatName l}, args) ->
-      let (env, args) = List.fold_right (fun arg (env,args) -> 
-        let (env, _, arg) = desugar_data_pat env arg in 
-        (env, arg::args)) args (env, []) in 
+      let (env, args) = List.fold_right (fun arg (env,args) ->
+        let (env, _, arg) = desugar_data_pat env arg in
+        (env, arg::args)) args (env, []) in
       let _ = fail_or (try_lookup_datacon env) l in
       let x = new_bvd (Some p.range) in
       (env, Inr(x, Typ_unknown), Pat_cons(l, args))
 
     | PatApp _ -> raise (Error ("Unexpected pattern", p.range))
 
-    | PatList pats -> 
-      let (env,pats) = List.fold_right (fun pat (env, pats) -> 
+    | PatList pats ->
+      let (env,pats) = List.fold_right (fun pat (env, pats) ->
         let (env,_,pat) = desugar_data_pat env pat in
         (env, pat::pats)) pats (env, []) in
       let pat = List.fold_right (fun hd tl -> Pat_cons(Const.cons_lid, [hd;tl])) pats (Pat_cons(Const.nil_lid, [])) in
-      let x = new_bvd (Some p.range) in 
+      let x = new_bvd (Some p.range) in
       (env, Inr(x, Typ_unknown), pat)
-      
-    | PatTuple(args) -> 
-      let env, args = List.fold_left (fun (env, pats) p -> 
-        let env, _, pat = desugar_data_pat env p in 
-        (env, pat::pats)) (env,[]) args in 
-      let args = List.rev args in 
-      let constr = fail_or (DesugarEnv.try_lookup_lid env) (lid_of_path [Util.strcat "MkTuple" (Util.string_of_int <| List.length args)] p.range) in 
-      let l = match constr.v with 
-        | Exp_fvar v -> v.v 
-        | _ -> raise Impos in 
-      let x = new_bvd (Some p.range) in 
+        
+    | PatTuple(args) ->
+      let env, args = List.fold_left (fun (env, pats) p ->
+        let env, _, pat = desugar_data_pat env p in
+        (env, pat::pats)) (env,[]) args in
+      let args = List.rev args in
+      let constr = fail_or (DesugarEnv.try_lookup_lid env) (lid_of_path [Util.strcat "MkTuple" (Util.string_of_int <| List.length args)] p.range) in
+      let l = match constr.v with
+        | Exp_fvar v -> v.v
+        | _ -> raise Impos in
+      let x = new_bvd (Some p.range) in
       (env, Inr(x, Typ_unknown), Pat_cons(l, args))
 
-    | PatRecord _ -> failwith "NYI" 
-
-and desugar_binding_pat env pat = 
-  let (env, binder, pat) = desugar_data_pat env pat in 
-  let pat = match pat with 
+    | PatRecord ([]) -> 
+      raise (Error ("Unexpected pattern", p.range))
+        
+    | PatRecord (fields) -> 
+      let (f, _) = List.hd fields in 
+      let record, _ = fail_or (try_lookup_record_by_field_name env) f in
+      let fields = fields |> List.map (fun (f, p) -> 
+        (fail_or (qualify_field_to_record env record) f, p)) in
+      let args = record.fields |> List.map (fun (f, _) -> 
+        match fields |> List.tryFind (fun (g, _) -> lid_equals f g) with 
+          | None -> mk_pattern PatWild p.range
+          | Some (_, p) -> p) in 
+      let app = mk_pattern (PatApp(mk_pattern (PatName record.constrname) p.range, args)) p.range in
+      desugar_data_pat env app
+        
+and desugar_binding_pat env pat =
+  let (env, binder, pat) = desugar_data_pat env pat in
+  let pat = match pat with
     | Pat_var _
     | Pat_tvar _ -> None
-    | _ -> Some pat in 
+    | _ -> Some pat in
   (env, binder, pat)
 
-and desugar_match_pat env pat = 
-  let (env, binder, pat) = desugar_data_pat env pat in 
+and desugar_match_pat env pat =
+  let (env, binder, pat) = desugar_data_pat env pat in
   (env, pat)
 
 and desugar_typ_or_exp (env:env) (t:term) : either<typ,exp> =
@@ -319,7 +338,7 @@ and desugar_typ_or_exp (env:env) (t:term) : either<typ,exp> =
   then Inl <| desugar_typ env t
   else Inr <| desugar_exp env t
 
-and desugar_exp (env:env) (top:term) : exp = 
+and desugar_exp (env:env) (top:term) : exp =
   let pos e = ewithpos e top.range in
   begin match top.term with
     | Const c -> pos <| Exp_constant c
@@ -335,7 +354,7 @@ and desugar_exp (env:env) (top:term) : exp =
           mk_app op args
       end
 
-    | Var l  
+    | Var l
     | Name l -> fail_or (DesugarEnv.try_lookup_lid env) l
 
     | Construct(l, args) ->
@@ -343,41 +362,42 @@ and desugar_exp (env:env) (top:term) : exp =
       let args = List.map (desugar_typ_or_exp env) args in
       pos <| Exp_constr_app(dt, args)
 
-    | Abs(binders, body) -> 
-      let ftv = List.fold_left (fun ftvs pat -> 
+    | Abs(binders, body) ->
+      let ftv = List.fold_left (fun ftvs pat ->
         match pat.pattern with
           | PatAscribed(_, t) -> free_type_vars env t@ftvs
-          | _ -> ftvs) [] binders in 
-      let ftv = sort_ftv ftv in 
-      let binders = (ftv |> List.map (fun a -> mk_pattern (PatTvar a) top.range))@binders in 
+          | _ -> ftvs) [] binders in
+      let ftv = sort_ftv ftv in
+      let binders = (ftv |> List.map (fun a -> mk_pattern (PatTvar a) top.range))@binders in
       let rec desugar_abs env a = match a.term with
-        | Abs(p::(q::_ as rest), body) ->
-          desugar_abs env  
+        | Abs((p::q::qtl), body) ->
+          let rest = q::qtl in
+          desugar_abs env
             (mk_term (Abs([p], mk_term (Abs(rest, body)) (Range.union_ranges q.range body.range) Expr))
                top.range Expr)
-        
+            
         | Abs([p], body) ->
-          let env, binder, pat = desugar_binding_pat env p in 
-          begin match binder with 
-            | Inl (a, k) -> 
-              let body = desugar_abs env body in 
+          let env, binder, pat = desugar_binding_pat env p in
+          begin match binder with
+            | Inl (a, k) ->
+              let body = desugar_abs env body in
               pos <| Exp_tabs(a, k, body)
-            | Inr (x, t) -> 
-              let body = desugar_exp env body in 
-              let body = match pat with 
+            | Inr (x, t) ->
+              let body = desugar_exp env body in
+              let body = match pat with
                 | None -> body
                 | Some pat -> ewithpos (Exp_match(bvd_to_exp x t, [(pat, None, body)])) body.p in
               pos <| Exp_abs(x, t, body)
           end
 
         | _ -> desugar_exp env a
-      in 
+      in
       desugar_abs env (mk_term (Abs(binders, body)) top.range top.level)
         
     | App({term=Var a}, arg) when (lid_equals a Const.assert_lid
                                    || lid_equals a Const.assume_lid) ->
       let phi = desugar_formula env arg in
-      pos <| Exp_app(pos <| Exp_tapp(fvar a (range_of_lid a), phi),  
+      pos <| Exp_app(pos <| Exp_tapp(fvar a (range_of_lid a), phi),
                      pos <| Exp_constant(Const_unit))
 
     | App(e, t) ->
@@ -388,44 +408,53 @@ and desugar_exp (env:env) (top:term) : exp =
     | Seq(t1, t2) ->
       desugar_exp env (mk_term (Let(false, [(mk_pattern PatWild t1.range,t1)], t2)) top.range Expr)
         
-    | Let(b, ((pat, _)::_ as bindings), body) when is_app_pattern pat ->
-      let funs = bindings |> List.map (fun (p, def) -> 
+    | Let(b, ((pat, _snd)::_tl), body) when is_app_pattern pat ->
+      let bindings = (pat, _snd)::_tl in
+      let funs = bindings |> List.map (fun (p, def) ->
         if not <| is_app_pattern p
         then raise (Error("Only functions may be defined recursively", p.range))
-        else (destruct_app_pattern p, def)) in 
-      let env', fnames = 
-        List.fold_left (fun (env, fnames) ((f, _, _), _) -> 
+        else (destruct_app_pattern p, def)) in
+      let env', fnames =
+        List.fold_left (fun (env, fnames) ((f, _, _), _) ->
           let env, fbvd = push_local_vbinding env f in
-          env, (fbvd::fnames)) (env, []) funs in 
+          env, (fbvd::fnames)) (env, []) funs in
       let fnames = List.rev fnames in
-      let desugar_one_def env ((_, args, result_t), def) = 
-        let def = match result_t with 
-          | None -> def 
+      let desugar_one_def env ((_, args, result_t), def) =
+        let def = match result_t with
+          | None -> def
           | Some t -> mk_term (Ascribed(def, t)) (Range.union_ranges t.range def.range) Expr in
         let def = mk_term (Abs(args, def)) top.range top.level in
         desugar_exp env def in
-      let defs = funs |> List.map (desugar_one_def (if b then env' else env)) in 
+      let defs = funs |> List.map (desugar_one_def (if b then env' else env)) in
       let lbs = List.map2 (fun fbvd def -> (fbvd, Typ_unknown, def)) fnames defs in
-      let body = desugar_exp env' body in 
+      let body = desugar_exp env' body in
       pos <| Exp_let(b, lbs, body)
           
     | Let(false, [(pat, t1)], t2) ->
       let t1 = desugar_exp env t1 in
       let env, binder, pat = desugar_binding_pat env pat in
-        begin match binder with
-          | Inl _ -> failwith "Unexpected type binder in let"
-          | Inr (x,t) -> 
-            let body = desugar_exp env t2 in
-            let body = match pat with 
-              | None -> body
-              | Some pat -> ewithpos (Exp_match(bvd_to_exp x t, [(pat, None, body)])) body.p in
-            pos <| Exp_let(false, [(x, t, t1)], body)
-        end
+      begin match binder with
+        | Inl _ -> failwith "Unexpected type binder in let"
+        | Inr (x,t) ->
+          let body = desugar_exp env t2 in
+          let body = match pat with
+            | None -> body
+            | Some pat -> ewithpos (Exp_match(bvd_to_exp x t, [(pat, None, body)])) body.p in
+          pos <| Exp_let(false, [(x, t, t1)], body)
+      end
 
     | If(t1, t2, t3) ->
       pos <| Exp_match(desugar_exp env t1,
                        [(Pat_constant (Const_bool true), None, desugar_exp env t2);
                         (Pat_constant (Const_bool false), None, desugar_exp env t3)])
+
+    | TryWith(e, branches) -> 
+      let r = top.range in 
+      let handler = mk_function branches r r in 
+      let body = mk_function [(mk_pattern (PatConst Const_unit) r, None, e)] r r in 
+      let a1 = mk_term (App(mk_term (Var Const.try_with_lid) r top.level, body)) r  top.level in 
+      let a2 = mk_term (App(a1, handler)) r top.level in 
+      desugar_exp env a2
 
     | Match(e, branches) ->
       let desugar_branch (pat, wopt, b) =
@@ -434,53 +463,58 @@ and desugar_exp (env:env) (top:term) : exp =
           | None -> None
           | Some e -> Some <| desugar_exp env e in
         let b = desugar_exp env b in
-        (pat, wopt, b) in 
+        (pat, wopt, b) in
       pos <| Exp_match(desugar_exp env e, List.map desugar_branch branches)
 
     | Ascribed(e, t) ->
       pos <| Exp_ascribed(desugar_exp env e, desugar_typ env t)
 
-    | Record(eopt, fields) -> 
-      let f, _ = List.hd fields in 
+    | Record(eopt, []) ->
+      raise (Error("Unexpected empty record", top.range))
+
+    | Record(eopt, fields) ->
+      let f, _ = List.hd fields in
       let record, _ = fail_or (try_lookup_record_by_field_name env) f in
-      let get_field xopt f = 
+      let get_field xopt f =
         let _, fn = Util.prefix f.lid in
-        let found = fields |> Util.find_opt (fun (g, _) -> 
-          let _, gn = Util.prefix g.lid in 
-          fn.idText = fn.idText) in 
-        match found with 
+        let found = fields |> Util.find_opt (fun (g, _) ->
+          let _, gn = Util.prefix g.lid in
+          fn.idText = fn.idText) in
+        match found with
           | Some (_, e) -> e
-          | None -> 
-            match xopt with 
-              | None -> 
+          | None ->
+            match xopt with
+              | None ->
                 raise (Error (Util.format1 "Field %s is missing" (text_of_lid f), top.range))
-              | Some x -> 
+              | Some x ->
                 mk_term (Project(x, f)) x.range x.level in
-      let recterm = match eopt with 
-        | None -> 
-          Construct(record.constrname, 
-                    record.fields |> List.map (fun (f, _) -> 
+      let recterm = match eopt with
+        | None ->
+          Construct(record.constrname,
+                    record.fields |> List.map (fun (f, _) ->
                       get_field None f))
             
-        | Some e -> 
-          let x = genident (Some e.range) in 
+        | Some e ->
+          let x = genident (Some e.range) in
           let xterm = mk_term (Var (lid_of_ids [x])) x.idRange Expr in
-          let record = Construct(record.constrname, 
-                                 record.fields |> List.map (fun (f, _) -> 
+          let record = Construct(record.constrname,
+                                 record.fields |> List.map (fun (f, _) ->
                                     get_field (Some xterm) f)) in
           Let(false, [(mk_pattern (PatVar x) x.idRange, e)], mk_term record top.range top.level) in
-      let recterm = mk_term recterm top.range top.level in 
+      let recterm = mk_term recterm top.range top.level in
       desugar_exp env recterm
         
-    | Project(e, f) -> 
-      let _, fieldname = fail_or (try_lookup_record_by_field_name env) f in 
-      let proj = mk_term (App(mk_term (Var fieldname) (range_of_lid f) Expr, e)) top.range top.level in 
+    | Project(e, f) ->
+      (* let _ = Util.print_string (Util.format1 "Looking up field name %s\n" (Print.sli f)) in *)
+      let _, fieldname = fail_or (try_lookup_record_by_field_name env) f in
+      (* let _ = Util.print_string (Util.format2 "resolved %s as %s\n" (Print.sli f) (Print.sli fieldname)) in *)
+      let proj = mk_term (App(mk_term (Var fieldname) (range_of_lid f) Expr, e)) top.range top.level in
       desugar_exp env proj
 
-    | Paren e -> 
-      desugar_exp env e 
+    | Paren e ->
+      desugar_exp env e
 
-    | _ -> 
+    | _ ->
       error "Unexpected term" top top.range
   end
   
@@ -489,7 +523,7 @@ and desugar_typ env (top:term) : typ =
   match top.term with
     | Wild -> pos <| Typ_unknown
 
-    | Op("*", [t1;t2]) when is_type env t1 -> 
+    | Op("*", [t1;t2]) when is_type env t1 ->
       desugar_typ env (mk_term (Sum([mk_binder (NoName t1) t1.range Type], t2)) top.range top.level)
       
     | Op("<>", args) ->
@@ -504,120 +538,122 @@ and desugar_typ env (top:term) : typ =
           mk_tapp (ftv l) args
       end
 
-    | Tvar a -> 
-      pos <| fail_or2 (try_lookup_typ_var env) a  
+    | Tvar a ->
+      pos <| fail_or2 (try_lookup_typ_var env) a
           
     | Var l
-    | Name l -> 
-      pos <| fail_or (try_lookup_typ_name env) l 
+    | Name l ->
+      pos <| fail_or (try_lookup_typ_name env) l
       
-    | Construct(l, args) -> 
-      let t = fail_or (try_lookup_typ_name env) l in 
-      let args = List.map (desugar_typ_or_exp env) args in 
+    | Construct(l, args) ->
+      let t = fail_or (try_lookup_typ_name env) l in
+      let args = List.map (desugar_typ_or_exp env) args in
       mk_tapp t args
 
-    | Abs(p::(q::_ as rest), body) -> 
-      let body = mk_term (Abs(rest, body)) (Range.union_ranges q.range body.range) top.level in 
+    | Abs(p::(q::_rest), body) ->
+      let rest = q::_rest in
+      let body = mk_term (Abs(rest, body)) (Range.union_ranges q.range body.range) top.level in
       let t = mk_term (Abs([p], body)) top.range top.level in
       desugar_typ env t
 
-    | Abs([p], body) -> 
-      let env, binder, pat = desugar_binding_pat env p in 
-      begin match pat with 
+    | Abs([p], body) ->
+      let env, binder, pat = desugar_binding_pat env p in
+      begin match pat with
         | Some _ -> raise (Error("Pattern matching at the type level is not supported", p.range))
-        | None -> 
-          let body = desugar_typ env body in 
+        | None ->
+          let body = desugar_typ env body in
           match binder with
             | Inl (a,k) -> pos <| Typ_tlam(a, k, body)
             | Inr (x,t) -> pos <| Typ_lam(x,t, body)
       end
 
-    | App(t1, t2) -> 
+    | App(t1, t2) ->
       let t1 = desugar_typ env t1 in
       let t2 = desugar_typ_or_exp env t2 in
       mk_tapp t1 [t2]
         
-    | Product([], t) -> 
+    | Product([], t) ->
       desugar_typ env t
       
-    | Product(b::(_::_ as bs), t) ->
+    | Product(b::(_bs::_bstl), t) ->
+      let bs = _bs::_bstl in
       desugar_typ env (mk_term (Product([b], mk_term (Product(bs, t)) top.range top.level)) top.range top.level)
 
     | Product([b], t) ->
       let tk = desugar_binder env b in
       let p = match tk with
-        | Inl(None, k) -> 
+        | Inl(None, k) ->
           let x = new_bvd (Some b.range) in
           Typ_univ(x, k, desugar_typ env t)
 
-        | Inl(Some x, k) -> 
-          let env, x = push_local_tbinding env x in 
+        | Inl(Some x, k) ->
+          let env, x = push_local_tbinding env x in
           Typ_univ(x, k, desugar_typ env t)
 
-        | Inr(None, t1) -> 
+        | Inr(None, t1) ->
           Typ_fun(None, t1, desugar_typ env t)
 
-        | Inr(Some x, t1) -> 
+        | Inr(Some x, t1) ->
           let env, x = push_local_vbinding env x in
           Typ_fun(Some x, t1, desugar_typ env t) in
       pos p
 
     | Refine(b,f) ->
       begin match desugar_exp_binder env b with
-        | (None, _) -> failwith "Missing binder in refinement" 
+        | (None, _) -> failwith "Missing binder in refinement"
         | (Some x, t) ->
-          let env, x = push_local_vbinding env x in 
+          let env, x = push_local_vbinding env x in
           let f = desugar_formula env f in
           pos <| Typ_refine(x, t, f)
       end
 
-    | Paren t -> 
+    | Paren t ->
       desugar_typ env t
 
-    | Ascribed(t,k) -> 
+    | Ascribed(t,k) ->
       pos <| Typ_ascribed(desugar_typ env t, desugar_kind env k)
 
-    | Sum(binders, t) -> 
-      let env, _, targs = List.fold_left (fun (env, tparams, typs) b -> 
-        let xopt, t = desugar_exp_binder env b in 
-        let env, x = match xopt with 
+    | Sum(binders, t) ->
+      let env, _, targs = List.fold_left (fun (env, tparams, typs) b ->
+        let xopt, t = desugar_exp_binder env b in
+        let env, x = match xopt with
           | None -> env, new_bvd (Some top.range)
-          | Some x -> push_local_vbinding env x in 
+          | Some x -> push_local_vbinding env x in
         (env, tparams@[Tparam_term(x, t)], typs@[close_with_lam tparams t]))
         (env, [], []) (binders@[mk_binder (NoName t) t.range Type]) in
       let tup = fail_or (try_lookup_typ_name env) (lid_of_path [Util.strcat "Tuple" (Util.string_of_int <| List.length targs)] top.range) in
-      pos <| List.fold_left (fun t1 t2 -> Typ_app(t1,t2)) tup targs 
+      pos <| List.fold_left (fun t1 t2 -> Typ_app(t1,t2)) tup targs
           
     | Record _ -> failwith "NYI: Records"
 
     | _ -> error "Expected a type" top top.range
 
-and desugar_kind env k : kind = 
-  match k.term with 
+and desugar_kind env k : kind =
+  match k.term with
     | Name {str="P"} -> Kind_prop
     | Name {str="S"} -> Kind_star
     | Name {str="E"} -> Kind_erasable
     | Wild           -> Kind_unknown
-    | Product([b], t) -> 
-      let tk = desugar_binder env b in 
-      begin match tk with 
-        | Inl(None, k) -> 
+    | Product([b], t) ->
+      let tk = desugar_binder env b in
+      begin match tk with
+        | Inl(None, k) ->
           Kind_tcon(None, k, desugar_kind env t)
 
-        | Inl(Some a, k) -> 
+        | Inl(Some a, k) ->
           let env, a = push_local_tbinding env a in
           Kind_tcon(Some a, k, desugar_kind env t)
 
-        | Inr(None, t0) -> 
+        | Inr(None, t0) ->
           Kind_dcon(None, t0, desugar_kind env t)
 
-        | Inr(Some x, t0) -> 
+        | Inr(Some x, t0) ->
           let env, x = push_local_vbinding env x in
           Kind_dcon(Some x, t0, desugar_kind env t)
       end
     | _ -> error "Unexpected term where kind was expected" k k.range
 
-and desugar_formula' env (f:term) : typ = 
+and desugar_formula' env (f:term) : typ =
   let connective s = match s with
     | "/\\"  -> Some Const.and_lid
     | "\\/"  -> Some Const.or_lid
@@ -625,42 +661,44 @@ and desugar_formula' env (f:term) : typ =
     | "<==>" -> Some Const.iff_lid
     | _ -> None in
   let pos t = Typ_meta (Meta_pos(t, f.range)) in
-  let desugar_quant (q:lident) (qt:lident) b pats body =  
-    let tk = desugar_binder env {b with level=Formula} in
-    match tk with 
-      | Inl(Some a,k) -> 
-        let env, a = push_local_tbinding env a in 
+  let desugar_quant (q:lident) (qt:lident) b pats body =
+    let tk = desugar_binder env ({b with level=Formula}) in
+    match tk with
+      | Inl(Some a,k) ->
+        let env, a = push_local_tbinding env a in
         let pats = List.map (desugar_typ_or_exp env) pats in
-        let body = desugar_formula env body in 
-        let body = match pats with 
+        let body = desugar_formula env body in
+        let body = match pats with
           | [] -> body
           | _ -> Typ_meta (Meta_pattern(body, pats)) in
-        let body = pos <| Typ_tlam(a, k, body) in 
+        let body = pos <| Typ_tlam(a, k, body) in
         pos <| mk_tapp (ftv (set_lid_range qt b.range)) [Inl body]
             
-      | Inr(Some x,t) -> 
-        let env, x = push_local_vbinding env x in 
+      | Inr(Some x,t) ->
+        let env, x = push_local_vbinding env x in
         let pats = List.map (desugar_typ_or_exp env) pats in
-        let body = desugar_formula env body in 
-        let body = match pats with 
+        let body = desugar_formula env body in
+        let body = match pats with
           | [] -> body
           | _ -> Typ_meta (Meta_pattern(body, pats)) in
-        let body = pos <| Typ_lam(x, t, body) in 
-        pos <| mk_tapp (ftv (set_lid_range q b.range)) [Inl body] 
+        let body = pos <| Typ_lam(x, t, body) in
+        pos <| mk_tapp (ftv (set_lid_range q b.range)) [Inl body]
 
       | _ -> raise Impos in
             
-  let push_quant q (binders:binder list) pats (body:term) = match binders with 
-    | b::(b'::_ as rest) -> 
-      let body = mk_term (q(rest, pats, body)) (Range.union_ranges b'.range body.range) Formula in 
+  let push_quant q (binders:binder list) pats (body:term) = match binders with
+    | b::(b'::_rest) ->
+      let rest = b'::_rest in
+      let body = mk_term (q(rest, pats, body)) (Range.union_ranges b'.range body.range) Formula in
       mk_term (q([b], [], body)) f.range Formula
     | _ -> raise Impos in
 
   match f.term with
-    | Op("=", ((hd::_) as args)) ->
+    | Op("=", ((hd::_args))) ->
+      let args = hd::_args in
       let args = List.map (desugar_typ_or_exp env) args in
-      let eq = 
-        if is_type env hd  
+      let eq =
+        if is_type env hd
         then ftv (set_lid_range Const.eqTyp_lid f.range)
         else ftv (set_lid_range Const.eq2_lid f.range) in
       mk_tapp eq args
@@ -668,64 +706,66 @@ and desugar_formula' env (f:term) : typ =
     | Op(s, args) ->
       begin match connective s, args with
         | Some conn, [_;_] ->
-          mk_tapp 
+          mk_tapp
             (ftv (set_lid_range conn f.range))
             (List.map (fun x -> Inl <| desugar_formula env x) args)
         | _ -> desugar_typ env f
       end
 
-    | App({term=Var l}, arg) when l.str = "not" ->
-      let arg = desugar_formula env arg in 
+    | App({term=Var l}, arg) when (l.str = "not") ->
+      let arg = desugar_formula env arg in
       mk_tapp (ftv (set_lid_range Const.not_lid f.range)) [Inl arg]
         
     | If(f1, f2, f3) ->
-      mk_tapp 
-        (ftv (set_lid_range Const.ite_lid f.range)) 
+      mk_tapp
+        (ftv (set_lid_range Const.ite_lid f.range))
         (List.map (fun x -> Inl <| desugar_typ env x) [f1;f2;f3])
 
-    | QForall((_::_::_ as binders), pats, body) ->
+    | QForall((_1::_2::_3), pats, body) ->
+      let binders = _1::_2::_3 in
       desugar_formula env (push_quant QForall binders pats body)
 
-    | QExists((_::_::_ as binders), pats, body) ->
+    | QExists((_1::_2::_3), pats, body) ->
+      let binders = _1::_2::_3 in
       desugar_formula env (push_quant QExists binders pats body)
         
     | QForall([b], pats, body) ->
-      desugar_quant Const.forall_lid Const.allTyp_lid b pats body 
+      desugar_quant Const.forall_lid Const.allTyp_lid b pats body
 
     | QExists([b], pats, body) ->
-      desugar_quant Const.exists_lid Const.allTyp_lid b pats body 
+      desugar_quant Const.exists_lid Const.allTyp_lid b pats body
 
-    | Paren f -> 
+    | Paren f ->
       desugar_formula env f
 
     | _ when is_type env f ->
       desugar_typ env f
 
-    | _ -> 
+    | _ ->
       error "Expected a formula" f f.range
 
-and desugar_formula env t = 
-  desugar_formula' {env with phase=Formula} t          
+and desugar_formula env t =
+  desugar_formula' ({env with phase=Formula}) t
 
-and desugar_binder env b = 
+and desugar_binder env b =
   if is_type_binder env b
   then Inl (desugar_type_binder env b)
   else Inr (desugar_exp_binder env b)
 
-and typars_of_binders env bs = 
-    let env, tpars = List.fold_left (fun (env, out) b -> 
-        let tk = desugar_binder env {b with level=Formula} in  (* typars follow the same binding conventions as formulas *)
-        match tk with 
-            | Inl(Some a,k) -> 
+and typars_of_binders env bs =
+    let env, tpars = List.fold_left (fun (env, out) b ->
+        let tk = desugar_binder env ({b with level=Formula}) in  (* typars follow the same binding conventions as formulas *)
+        match tk with
+            | Inl(Some a,k) ->
                 let env, a = push_local_tbinding env a in
                 (env, Tparam_typ(a,k)::out)
-            | Inr(Some x,t) -> 
+            | Inr(Some x,t) ->
                 let env, x = push_local_vbinding env x in
                 (env, Tparam_term(x,t)::out)
             | _ -> raise (Error ("Unexpected binder", b.range))) (env, []) bs in
     env, List.rev tpars
 
-and desugar_exp_binder env b = match b.binder with 
+and desugar_exp_binder env b = match b.binder with
   | Annotated(x, t) -> Some x, desugar_typ env t
   | TVariable t -> None, fail_or2 (try_lookup_typ_var env) t
   | NoName t -> None, desugar_typ env t
@@ -740,19 +780,19 @@ and desugar_type_binder env b = match b.binder with
 
 let logic_tag = function
   | LogicTag l -> [l]
-  | _ -> [] 
+  | _ -> []
 
 let logic_tags q = List.collect logic_tag q
 
-let mk_data_ops env = function 
-  | Sig_datacon(lid, t) -> 
+let mk_data_ops env = function
+  | Sig_datacon(lid, t) ->
     let args, tconstr = collect_formals t in
-    let argpats = args |> List.map (function 
-      | Inr(Some x,_) -> Pat_var x 
+    let argpats = args |> List.map (function
+      | Inr(Some x,_) -> Pat_var x
       | Inr(None,targ) -> Pat_var (new_bvd (Some (range_of_lid lid)))
       | Inl(a,_) -> Pat_tvar a) in
-    let freetv, freexv  = freevars_typ tconstr in 
-    let freevars = (List.map Inl freetv)@(List.map Inr freexv) in 
+    let freetv, freexv  = freevars_typ tconstr in
+    let freevars = (List.map Inl freetv)@(List.map Inr freexv) in
     let formal = new_bvd (Some <| range_of_lid lid) in
     let formal_exp = bvd_to_exp formal tconstr in
     let rec build_exp freevars e = match freevars with
@@ -765,41 +805,41 @@ let mk_data_ops env = function
       | [] -> Typ_fun(Some formal, tconstr, t) in
     let rec build_kind freevars k = match freevars with
       | Inl a::rest -> Kind_tcon(Some a.v, a.sort, build_kind rest k)
-      | Inr x::rest -> Kind_dcon(Some x.v, x.sort, build_kind rest k) 
+      | Inr x::rest -> Kind_dcon(Some x.v, x.sort, build_kind rest k)
       | [] -> Kind_dcon(Some formal, tconstr, k) in
-    let build_exp  = build_exp freevars in 
-    let build_typ  = build_typ freevars in 
+    let build_exp  = build_exp freevars in
+    let build_typ  = build_typ freevars in
     let build_kind = build_kind freevars in
-    let rec aux subst fields t = match compress t with 
-      | Typ_fun(Some x, t1, t2) -> 
+    let rec aux subst fields t = match compress t with
+      | Typ_fun(Some x, t1, t2) ->
         let field_name = lid_of_ids (lid.lid @ [x.ppname]) in
-        let t = build_typ t1 in 
+        let t = build_typ t1 in
         let body = ewithpos (Exp_match(formal_exp, [(Pat_cons(lid, argpats), None, bvd_to_exp x t1)])) x.ppname.idRange in
-        let sigs = 
+        let sigs =
           [Sig_val_decl(field_name, t);
            Sig_let([(field_name, t, build_exp body)], false)] in
         (* let _ = Util.print_string (Util.format1 "adding value projector %s\n" field_name.str) in *)
         let subst = Inr(x, mk_app (fvar field_name (range_of_lid field_name)) [Inr formal_exp])::subst in
-        let t2 = subst_typ subst t2 in 
+        let t2 = subst_typ subst t2 in
         aux subst (fields@sigs) t2
           
-      | Typ_univ(a, k, t2) -> 
+      | Typ_univ(a, k, t2) ->
         let field_name = lid_of_ids (lid.lid @ [a.ppname]) in
         let sigs = Sig_tycon(field_name, [], build_kind k, [], [], [Logic_projector]) in
         (* let _ = Util.print_string (Util.format1 "adding type projector %s\n" field_name.str) in *)
         let subst = Inl(a, mk_tapp (ftv field_name) [Inr formal_exp])::subst in
-        let t2 = subst_typ subst t2 in 
+        let t2 = subst_typ subst t2 in
         aux subst (fields@[sigs]) t2
 
-      | _ -> fields in 
+      | _ -> fields in
     
-    aux [] [] t 
+    aux [] [] t
   | _ -> []
 
 let rec desugar_tycon env quals tcs : (env * sigelts) =
   let tycon_id = function
-    | TyconAbstract(id, _, _) 
-    | TyconAbbrev(id, _, _, _) 
+    | TyconAbstract(id, _, _)
+    | TyconAbbrev(id, _, _, _)
     | TyconRecord(id, _, _, _)
     | TyconVariant(id, _, _, _) -> id in
   let binder_to_term b = match b.binder with
@@ -807,22 +847,23 @@ let rec desugar_tycon env quals tcs : (env * sigelts) =
     | Variable x -> mk_term (Var (lid_of_ids [x])) x.idRange Expr
     | TAnnotated(a, _)
     | TVariable a -> mk_term (Tvar a) a.idRange Type
-    | NoName t -> t in 
-  let apply_binders t binders = 
+    | NoName t -> t in
+  let apply_binders t binders =
     List.fold_left (fun out b -> mk_term (App(out, binder_to_term b)) out.range out.level)
       t binders in
   let tycon_record_as_variant = function
     | TyconRecord(id, parms, kopt, fields) ->
       let constrName = mk_ident("Mk" ^ id.idText, id.idRange) in
-      let fields = List.map (fun (x,t) -> mk_binder (Annotated(x,t)) x.idRange Expr) fields in 
+      let fields = List.map (fun (x,t) -> mk_binder (Annotated(x,t)) x.idRange Expr) fields in
       let result = apply_binders (mk_term (Var (lid_of_ids [id])) id.idRange Type) parms in
-      let constrTyp = mk_term (Product(fields, result)) id.idRange Type in 
+      let constrTyp = mk_term (Product(fields, result)) id.idRange Type in
+      (* let _ = Util.print_string (Util.format2 "Translated record %s to constructor %s\n" (id.idText) (term_to_string constrTyp)) in *)
       TyconVariant(id, parms, kopt, [(constrName, constrTyp, false)])
     | _ -> raise Impos in
-  let desugar_abstract_tc env mutuals = function
+  let desugar_abstract_tc quals env mutuals = function
     | TyconAbstract(id, binders, kopt) ->
-      let env', typars = typars_of_binders env binders in 
-      let k = match kopt with 
+      let env', typars = typars_of_binders env binders in
+      let k = match kopt with
         | None -> Kind_star
         | Some k -> desugar_kind env' k in
       let tconstr = apply_binders (mk_term (Var (lid_of_ids [id])) id.idRange Type) binders in
@@ -837,63 +878,69 @@ let rec desugar_tycon env quals tcs : (env * sigelts) =
     | Tparam_typ(a,_) -> push_btvdef env a in
   let push_tparams = List.fold_left push_tparam in
   match tcs with
-    | [TyconAbstract _ as tc] ->
-        let _, _, se, _ = desugar_abstract_tc env [] tc in
-        let env = push_sigelt env se in 
+    | [TyconAbstract _] ->
+        let tc = List.hd tcs in
+        let _, _, se, _ = desugar_abstract_tc quals env [] tc in
+        let env = push_sigelt env se in
         (* let _ = pr "Pushed %s\n" (text_of_lid (qualify env (tycon_id tc))) in *)
         env, [se]
 
     | [TyconAbbrev(id, binders, kopt, t)] ->
-        let env', typars = typars_of_binders env binders in 
-        let k = match kopt with 
+        let env', typars = typars_of_binders env binders in
+        let k = match kopt with
             | None -> Kind_star
             | Some k -> desugar_kind env' k in
-        let t = desugar_typ env' t in 
+        let t = desugar_typ env' t in
         let se = Sig_typ_abbrev(qualify env id, typars, k, t) in
-        let env = push_sigelt env se in 
+        let env = push_sigelt env se in
         env, [se]
 
-    | [TyconRecord _ as trec] -> 
+    | [TyconRecord _] ->
+      let trec = List.hd tcs in
       desugar_tycon env (LogicTag Logic_record::quals) [tycon_record_as_variant trec]
 
-    |  _::_ -> 
-      let env0 = env in 
-      let mutuals = List.map (fun x -> qualify env <| tycon_id x) tcs in 
-      let rec collect_tcs (env, tcs) = function
-        | TyconRecord _ as trec -> 
-          collect_tcs (env, tcs) (tycon_record_as_variant trec)
-        | TyconVariant(id, binders, kopt, constructors) -> 
-          let env, (_, tps), se, tconstr = desugar_abstract_tc env mutuals (TyconAbstract(id, binders, kopt)) in
-          env, Inl(se, tps, constructors, tconstr)::tcs
-        | TyconAbbrev(id, binders, kopt, t) -> 
-          let env, (_, tps), se, tconstr = desugar_abstract_tc env mutuals (TyconAbstract(id, binders, kopt)) in
-          env, Inr(se, tps, t)::tcs
-        | _ -> failwith "Unrecognized mutual type definition" in 
-      let env, tcs = List.fold_left collect_tcs (env, []) tcs in 
-      let tcs = List.rev tcs in 
+    |  _::_ ->
+      let env0 = env in
+      let mutuals = List.map (fun x -> qualify env <| tycon_id x) tcs in
+      let rec collect_tcs (env, tcs, quals) tc = match tc with
+        | TyconRecord _ ->
+          let trec = tc in
+          collect_tcs (env, tcs, LogicTag Logic_record::quals) (tycon_record_as_variant trec)
+        | TyconVariant(id, binders, kopt, constructors) ->
+          let env, (_, tps), se, tconstr = desugar_abstract_tc quals env mutuals (TyconAbstract(id, binders, kopt)) in
+          env, Inl(se, tps, constructors, tconstr)::tcs, quals
+        | TyconAbbrev(id, binders, kopt, t) ->
+          let env, (_, tps), se, tconstr = desugar_abstract_tc quals env mutuals (TyconAbstract(id, binders, kopt)) in
+          env, Inr(se, tps, t)::tcs, quals
+        | _ -> failwith "Unrecognized mutual type definition" in
+      let env, tcs, quals = List.fold_left collect_tcs (env, [], quals) tcs in
+      let tcs = List.rev tcs in
       let sigelts = tcs |> List.collect (function
-        | Inr(Sig_tycon(id, tpars, k, _, _, _), tps, t) -> 
+        | Inr(Sig_tycon(id, tpars, k, _, _, _), tps, t) ->
           let env_tps = push_tparams env tps in
           let t = desugar_typ env_tps t in
           [Sig_typ_abbrev(id, tpars, k, t)]
             
-        | Inl (Sig_tycon(id, tpars, k, mutuals, _, tags), tps, constrs, tconstr) -> 
+        | Inl (Sig_tycon(id, tpars, k, mutuals, _, tags), tps, constrs, tconstr) ->
           let env_tps = push_tparams env tps in
           let constrNames, constrs = List.split <|
-              (constrs |> List.map (fun (id, t, of_notation) -> 
-                let t = 
+              (constrs |> List.map (fun (id, t, of_notation) ->
+                let t =
                   if of_notation
                   then mk_term (Product([mk_binder (NoName t) t.range t.level], tconstr)) t.range t.level
-                  else t in 
+                  else t in
                 let t = desugar_typ env_tps (close env_tps t) in
-                let name = qualify env id in 
-                (name, Sig_datacon(name, close_typ tps t)))) in 
+                let name = qualify env id in
+                (name, Sig_datacon(name, close_typ tps t)))) in
               Sig_tycon(id, tpars, k, mutuals, constrNames, tags)::constrs
-        | _ -> raise Impos) in 
+        | _ -> raise Impos) in
       let bundle = Sig_bundle sigelts in
       let env = push_sigelt env0 bundle in
-      let data_ops = 
-        if List.exists (function Logic_data | Logic_record -> true | _ -> false) (logic_tags quals) 
+      let data_ops =
+        if logic_tags quals |> Util.for_some (function
+          | Logic_data
+          | Logic_record -> true
+          | _ -> false)
         then sigelts |> List.collect (mk_data_ops env)
         else [] in
       let env = List.fold_left push_sigelt env data_ops in
@@ -902,19 +949,19 @@ let rec desugar_tycon env quals tcs : (env * sigelts) =
     | [] -> raise Impos
            
 let desugar_decl env (d:decl) : (env * sigelts) = match d.decl with
-  | Open lid -> 
-    let env = DesugarEnv.push_namespace env lid in 
+  | Open lid ->
+    let env = DesugarEnv.push_namespace env lid in
     env, []
   
   | Tycon(qual, tcs) ->
     desugar_tycon env [qual] tcs
           
   | ToplevelLet(isrec, lets) ->
-    begin match desugar_exp env (mk_term (Let(isrec, lets, mk_term (Const Const_unit) d.range Expr)) d.range Expr) with 
-        | {v=Exp_let(_, lbs, _)} -> 
+    begin match desugar_exp env (mk_term (Let(isrec, lets, mk_term (Const Const_unit) d.range Expr)) d.range Expr) with
+        | {v=Exp_let(_, lbs, _)} ->
           let lbs = List.map (fun (x, t, e) -> (qualify env x.ppname, t, e)) lbs in
           let s = Sig_let(lbs,isrec) in
-          let env = push_sigelt env s in 
+          let env = push_sigelt env s in
           env, [s]
         | _ -> failwith "Desugaring a let did not produce a let"
     end
@@ -929,22 +976,22 @@ let desugar_decl env (d:decl) : (env * sigelts) = match d.decl with
       env, [Sig_assume(qualify env id, f, Public, Assumption)]
 
   | Val(NoQual, id, t) ->
-      let t = desugar_typ env (close env t) in 
-      let se = Sig_val_decl(qualify env id, t) in 
-      let env = push_sigelt env se in 
+      let t = desugar_typ env (close env t) in
+      let se = Sig_val_decl(qualify env id, t) in
+      let env = push_sigelt env se in
       env, [se]
 
   | Val(LogicTag Logic_val, id, t) ->
-      let t = desugar_typ env (close env t) in 
-      let se = Sig_logic_function(qualify env id, t, []) in 
-      let env = push_sigelt env se in 
+      let t = desugar_typ env (close env t) in
+      let se = Sig_logic_function(qualify env id, t, []) in
+      let env = push_sigelt env se in
       env, [se]
         
-  | Exception(id, term) -> 
-    let t = desugar_typ env term in 
+  | Exception(id, term) ->
+    let t = desugar_typ env term in
     let t = Typ_fun(None, t, fail_or (try_lookup_typ_name env) Const.exn_lid) in
-    let se = Sig_datacon(qualify env id, t) in 
-    let env = push_sigelt env se in 
+    let se = Sig_datacon(qualify env id, t) in
+    let env = push_sigelt env se in
     env, [se]
 
   | _ -> raise (Error("Unexpected declaration", d.range))
@@ -952,22 +999,19 @@ let desugar_decl env (d:decl) : (env * sigelts) = match d.decl with
 let desugar_modul env (m:AST.modul) : env * Syntax.modul = match m with
   | Module(mname, decls) ->
       let env = DesugarEnv.prepare_module env mname in
-      let env, sigelts = List.fold_left (fun (env, sigelts) d -> 
-        let env, se = desugar_decl env d in 
-        env, sigelts@se) (env, []) decls in 
-      let modul = { 
+      let env, sigelts = List.fold_left (fun (env, sigelts) d ->
+        let env, se = desugar_decl env d in
+        env, sigelts@se) (env, []) decls in
+      let modul = {
         name = mname;
-        declarations = sigelts; 
+        declarations = sigelts;
         exports = []
       } in
-      let env = DesugarEnv.finish_module env modul in 
+      let env = DesugarEnv.finish_module env modul in
       env, modul
-          
   
 let desugar_file env (pragmas, ms) =
-  let env, mods = List.fold_left (fun (env, mods) m -> 
+  let env, mods = List.fold_left (fun (env, mods) m ->
     let env, m = desugar_modul env m in
     env, m::mods) (env, []) ms in
   env, List.rev mods
-            
-
