src/parser/driver.fs
@@ -19,39 +19,18 @@ module Microsoft.FStar.Parser.Driver
 open Microsoft.FStar
 open Microsoft.FStar.Parser
 open Microsoft.FStar.Parser.AST
-open Microsoft.FStar.Parser.Lexhelp
 open Microsoft.FStar.Parser.Parse
 open Util
 
 let print_error msg r = 
-  Printf.printf "ERROR %s: %s\n" (Range.string_of_range r) msg
+  Util.print_string (Util.format2 "ERROR %s: %s\n" (Range.string_of_range r) msg)
 
 let parse env fn =
-  Parse.warningHandler := (function 
-    | Lexhelp.ReservedKeyword(m,s) -> Printf.printf "%s:%s" (Range.string_of_range s) m
-    | e -> Printf.printf "Warning: %A\n" e);
-
-  let filename,sr = match fn with 
-    | Inl (filename:string) -> filename, 
-      (try new System.IO.StreamReader(filename) :> System.IO.TextReader
-       with _ -> raise (Absyn.Syntax.Err (Util.format1 "Unable to open file: %s" filename)))
-    | Inr (s:string) -> "<input>", new System.IO.StringReader(s) :> System.IO.TextReader in
-
-  let lexbuf = Microsoft.FSharp.Text.Lexing.LexBuffer<char>.FromTextReader(sr) in
-  resetLexbufPos filename lexbuf;
-  let lexargs = mkLexargs ((fun () -> "."), filename) in 
-  let lexer = LexFStar.token lexargs in 
-    try
-      let ast = Parse.file lexer lexbuf in 
-      Desugar.desugar_file env ast
-    with 
-      | Absyn.Syntax.Error(msg, r) -> 
-        print_error msg r;
-        exit 0 
-      | e ->
-        let pos = lexbuf.EndPos in
-        Printf.printf "ERROR: Syntax error near line %d, character %d in file %s\n" (pos.pos_lnum) (pos.pos_cnum - pos.pos_bol) filename;
-        exit 0
+  match ParseIt.parse_file fn with 
+    | Inl ast -> Desugar.desugar_file env ast
+    | Inr msg -> 
+      Util.print_string msg;
+      exit 0
 
 let parse_files files = 
   let _, mods = List.fold_left (fun (env,mods) fn -> 
@@ -59,8 +38,3 @@ let parse_files files =
     (env, m::mods)) (DesugarEnv.empty_env(), []) files in 
   List.rev mods |> List.flatten
   
-#if TEST
-let _ =
-    let files = List.tl <| List.ofArray Sys.argv in 
-    parse_files files   
-#endif 
