src/parser/parseit.fs
@@ -1,0 +1,37 @@
+module Microsoft.FStar.Parser.ParseIt
+open Microsoft.FStar
+open Microsoft.FStar.Util
+
+let resetLexbufPos filename (lexbuf: Microsoft.FSharp.Text.Lexing.LexBuffer<char>) = 
+  lexbuf.EndPos <- {lexbuf.EndPos with 
+    pos_fname= Range.encode_file filename; 
+    pos_cnum=0;
+    pos_lnum=1 }
+
+let parse_file fn = 
+  Parse.warningHandler := (function
+    | Lexhelp.ReservedKeyword(m,s) -> Printf.printf "%s:%s" (Range.string_of_range s) m
+    | e -> Printf.printf "Warning: %A\n" e);
+  
+  let filename,sr = match fn with 
+    | Inl (filename:string) -> filename, 
+      (try new System.IO.StreamReader(filename) :> System.IO.TextReader
+       with _ -> raise (Absyn.Syntax.Err (Util.format1 "Unable to open file: %s" filename)))
+    | Inr (s:string) -> "<input>", new System.IO.StringReader(s) :> System.IO.TextReader in
+
+  let lexbuf = Microsoft.FSharp.Text.Lexing.LexBuffer<char>.FromTextReader(sr) in
+  resetLexbufPos filename lexbuf;
+  let lexargs = Lexhelp.mkLexargs ((fun () -> "."), filename) in 
+  let lexer = LexFStar.token lexargs in 
+  try
+    Inl (Parse.file lexer lexbuf)
+  with 
+    | Absyn.Syntax.Error(msg, r) -> 
+      let msg = Util.format2 "ERROR %s: %s\n" (Range.string_of_range r) msg in
+      Inr msg
+    | e ->
+      let pos = lexbuf.EndPos in
+      Inr  (Util.format3 "ERROR: Syntax error near line %s, character %s in file %s\n" 
+              (Util.string_of_int pos.pos_lnum) 
+              (Util.string_of_int (pos.pos_cnum - pos.pos_bol))
+              filename)
