src/parser/parseit.fsi
@@ -1,0 +1,5 @@
+module Microsoft.FStar.Parser.ParseIt
+open Microsoft.FStar.Parser
+open Microsoft.FStar.Util
+
+val parse_file: either<string,string> -> either<AST.file, string>
