src/basic/bytes.fst
@@ -1,0 +1,19 @@
+module Microsoft.FStar.Bytes
+
+type bytes
+val length : bytes -> int
+val get: bytes -> int -> int
+val zero_create : int -> bytes
+val of_intarray: array<int> -> bytes
+val string_as_unicode_bytes: string -> bytes
+val unicode_bytes_as_string: bytes -> string
+val utf8_bytes_as_string: bytes -> string
+val append: bytes -> bytes -> bytes
+val make: (int -> int) -> int -> bytes
+val for_range: bytes -> int -> int -> (int -> unit) -> unit
+
+type bytebuf
+val create: int -> bytebuf
+val close : bytebuf -> bytes
+val emit_int_as_byte: bytebuf -> int -> unit
+val emit_bytes: bytebuf -> bytes -> unit
